---
title: "Data607 - Homework14"
author: "Amit Kapoor"
date: "5/7/2020"
output:
  html_document: default
  pdf_document: default
---

```{r setup, include=FALSE}
knitr::opts_chunk$set(echo = TRUE)
```

This week, we'll work out some Taylor Series expansions of popular functions

* f(x) = 1 / (1-x)
* f(x) = e^x
* f(x) = ln(1 + x)

For each function, only consider its valid ranges as indicated in the notes when you are
computing the Taylor Series expansion. Please submit your assignment as a R-Markdown
document.

Taylor series is defined as 

$$f(x)\quad =\sum _{n=0 }^{\infty}{\frac {f^{n}(a)}{n!}}(x-a)^{n}\quad$$
    
### 1. f(x) = 1 / (1-x)

Lets find derivatives,

$$f^0(c) = \frac{1}{(1-c)}$$
$$f^{'}(c) = \frac{1}{(1-c)^2}$$
$$f^{''}(c) = \frac{2}{(1-c)^3}$$

$$f^{'''}(c) = \frac{6}{(1-c)^4}$$

$$f^{''''}(c) = \frac{24}{(1-c)^5}$$

As per definition, 


$$ f(x) = \frac{1}{(1-c)0!}(x-c)^0+\frac{1}{(1-c)^21!}(x-c)^1+\frac{2}{(1-c)^32!}(x-c)^2+\frac{6}{(1-c)^43!}(x-c)^3+ ...$$
$$ = \frac{1}{(1-c)}+\frac{1}{(1-c)^2}(x-c)+\frac{2!}{(1-c)^32!}(x-c)^2+\frac{3!}{(1-c)^43!}(x-c)^3+ ...$$
$$ = \frac{1}{(1-c)}+\frac{1}{(1-c)^2}(x-c)+\frac{1}{(1-c)^3}(x-c)^2+\frac{1}{(1-c)^4}(x-c)^3+ ...$$
$$ =\sum _{n=0 }^{\infty}\frac {1}{(1-c)^{n+1}}(x-c)^n$$

Using Maclaurin series c = 0,

$$f(x) =\sum _{n=0 }^{\infty}x^n = 1+x+x^2+x^3+x^4+ ..... $$

The series converges in the interval (-1,1)



### 2. f(x) = e^x

Lets find derivatives,

$$f^0(c) = e^c$$
$$f^{'}(c) = e^c$$
$$f^{''}(c) = e^c$$
$$f^{'''}(c) = e^c$$
$$f^{''''}(c) = e^c$$


As per definition, 


$$ f(x) = \frac{e^c}{0!}(x-c)^0+\frac{e^c}{1!}(x-c)^1+\frac{e^c}{2!}(x-c)^2+\frac{e^c}{3!}(x-c)^4+ ...$$

$$ =e^c \sum _{n=0 }^{\infty}\frac {(x-c)^n}{n!}$$

Using Maclaurin series c = 0,

$$f(x) =\sum _{n=0 }^{\infty}\frac {x^n}{n!} = 1+x+\frac{x^2}{2}+\frac{x^3}{6}+\frac{x^4}{24}+ ..... $$


Test ratio

$$ \frac {a_{n+1}}{a_n} = \frac {x^{n+1}}{(n+1)!} * \frac {n!}{x^n} = \frac {x}{n+1}$$


$$L = \lim_{n\to\infty} \frac {x}{n+1} = 0$$

Hence the series converges for $\forall$ x in the range (-$\infty$, $\infty$)

### 3. f(x) = ln(1 + x)

Lets find derivatives,

$$f^0(c) = ln(1 + c)$$

$$f^{'}(c) = \frac{1}{(c+1)}$$

$$f^{''}(c) = -\frac{1}{(c+1)^2}$$

$$f^{'''}(c) = \frac{2}{(c+1)^3}$$

$$f^{''}(c) = -\frac{6}{(c+1)^4}$$


As per definition, 

$$ f(x) = \frac{ln(1+c)}{0!}(x-c)^0+\frac{1}{(c+1)1!}(x-c)^1-\frac{1}{(c+1)^22!}(x-c)^2+\frac{2}{(c+1)^33!}(x-c)^3-\frac{6}{(c+1)^44!}(x-c)^4+ ...$$

$$= ln(1+c)+\frac{1}{(c+1)}(x-c)-\frac{1!}{(c+1)^22*1!}(x-c)^2+\frac{2!}{(c+1)^33*2!}(x-c)^3-\frac{3!}{(c+1)^44*3!}(x-c)^4+ ...$$

$$= ln(1+c)+\frac{1}{(c+1)}(x-c)-\frac{1}{2(c+1)^2}(x-c)^2+\frac{1}{3(c+1)^3}(x-c)^3-\frac{1}{4(c+1)^4}(x-c)^4+ ...$$

$$= ln(1+c)+\sum _{n=0 }^{\infty}(-1)^{n+1}\frac {(x-c)^n}{n(c+1)^n!}$$

Using Maclaurin series c = 0,

$$f(x) =\sum _{n=0 }^{\infty}(-1)^{n+1}\frac {x^n}{n} = x-\frac{x^2}{2}+\frac{x^3}{3}-\frac{x^4}{4}+ ..... $$

Test ratio

$$ \frac {a_{n+1}}{a_n} = \frac {(-1)^{n+1+1}x^{n+1}}{(n+1)} * \frac {n}{(-1)^{n+1}x^{n}} = \frac {-xn}{n+1}$$

$$L = \lim_{n\to\infty} | \frac {-xn}{n+1}| = |x|$$

Hence the series converges for x in the range (-1, 1).




